src/GraphConformance.v
@@ -9,6 +9,7 @@ Unset Printing Implicit Defensive.
 Require Import String.
 Require Import QString.
 
+Require Import Value.
 
 Require Import Schema.
 Require Import SchemaWellFormedness.
@@ -47,7 +48,7 @@ Require Import Graph.
 Section Conformance.
 
 
-  Variables (Value : eqType).
+  Variable (Scalar : eqType).
 
   (** ---- *)
   (** ** Auxiliary definitions 
@@ -57,8 +58,8 @@ Section Conformance.
   (** ---- *)
   Section GraphAux.
 
-    Variable (graph :  @graphQLGraph Value).
-    Implicit Type edge : @node Value * @label Value * @node Value.
+    Variable (graph :  @graphQLGraph Scalar).
+    Implicit Type edge : @node Scalar * @label Scalar * @node Scalar.
 
     
     
@@ -140,7 +141,8 @@ Section Conformance.
 
   Section Predicates.
 
-    Variable (s : @wfGraphQLSchema Value).
+    Variables (s : wfGraphQLSchema)
+              (is_valid_scalar_value : graphQLSchema -> Name -> Scalar -> bool).
 
 
       
@@ -151,7 +153,7 @@ Section Conformance.
 
       This predicate checks that a Graph's root node must have the same type as the Schema's query type.
      **)
-    Definition root_type_conforms (root : @node Value) : bool := (root).(ntype) == s.(query_type).
+    Definition root_type_conforms (root : @node Scalar) : bool := (root).(ntype) == s.(query_type).
     
 
     (** ---- *)
@@ -168,10 +170,10 @@ Section Conformance.
      **)
     
     Definition arguments_conform ty (f : label) : bool :=
-      let argument_conforms (fname : Name) (arg : Name * Value) : bool :=
+      let argument_conforms (fname : Name) (arg : Name * @Value Scalar) : bool :=
           let: (argname, value) := arg in
           match lookup_argument_in_type_and_field s ty fname argname with
-          | Some field_arg => s.(is_valid_value) field_arg.(argtype) value    (* If the argument is declared then check its value's type *)
+          | Some field_arg => is_valid_value s is_valid_scalar_value field_arg.(argtype) value    (* If the argument is declared then check its value's type *)
           | _ => false
           end
       in
@@ -205,7 +207,7 @@ Section Conformance.
        these types in a graph. More is discussed in the corresponding paper.     
      **)    
     Definition edges_conform graph :=
-      let edge_conforms (edge : node * label * @node Value) : bool :=
+      let edge_conforms (edge : node * label * @node Scalar) : bool :=
           let: (src, label, target) := edge in
           match lookup_field_in_type s src.(ntype) label.(lname) with
           | Some fdef =>
@@ -238,10 +240,10 @@ Section Conformance.
           (If a field has an Int type then the value should represent an integer value).
        
      **)    
-    Definition nodes_conform (nodes : seq (@node Value)) :=
-      let property_conforms ty (fd : label * Value) : bool :=
+    Definition nodes_conform (nodes : seq (@node Scalar)) :=
+      let property_conforms ty (fd : label * @Value Scalar) : bool :=
           match lookup_field_in_type s ty fd.1.(lname) with
-          | Some fdef => arguments_conform ty fd.1 && s.(is_valid_value) fdef.(return_type) fd.2
+          | Some fdef => arguments_conform ty fd.1 && is_valid_value s is_valid_scalar_value fdef.(return_type) fd.2
           | _ => false
           end
       in
@@ -252,6 +254,8 @@ Section Conformance.
       all node_conforms nodes.
 
   End Predicates.
+
+  Variable (is_valid_scalar_value : graphQLSchema -> Name -> Scalar -> bool).
 
   (** ---- *)
   (** *** Conforming graph *)
@@ -266,10 +270,12 @@ Section Conformance.
      - Its nodes conform to the Schema.
 
    *)
-  Definition is_a_conforming_graph (s : wfGraphQLSchema) (graph : graphQLGraph) : bool :=
+  Definition is_a_conforming_graph (s : wfGraphQLSchema)
+             (is_valid_scalar_value : graphQLSchema -> Name -> Scalar -> bool)
+             (graph : @graphQLGraph Scalar) : bool :=
     [&& root_type_conforms s graph.(root),
-        edges_conform s graph &
-        nodes_conform s graph.(nodes)].
+        edges_conform s is_valid_scalar_value graph &
+        nodes_conform s is_valid_scalar_value graph.(nodes)].
 
   
   (** ---- *)
@@ -279,12 +285,14 @@ Section Conformance.
      A conformed GraphQL graph is a graph which conforms to a given schema.
 
    **)
-  Record conformedGraph (s : wfGraphQLSchema) := ConformedGraph {
-                                                    graph : graphQLGraph;
-                                                    _ : is_a_conforming_graph s graph
-                                                  }.
+  Record conformedGraph (s : wfGraphQLSchema)
+         (is_valid_scalar_value : graphQLSchema -> Name -> Scalar -> bool) :=
+    ConformedGraph {
+        graph : graphQLGraph;
+        _ : is_a_conforming_graph s is_valid_scalar_value graph
+      }.
 
-  Coercion graph_of_conformed_graph s (g : conformedGraph s) := let: ConformedGraph g _ := g in g.
+  Coercion graph_of_conformed_graph s vsv (g : conformedGraph s vsv) := let: ConformedGraph g _ := g in g.
 
 
                
