src/SchemaAux.v
@@ -10,6 +10,7 @@ From Equations Require Import Equations.
 Require Import String.
 Require Import QString.
 
+Require Import Value.
 
 Require Import Schema.
 Require Import SeqExtra.
@@ -270,6 +271,31 @@ Section SchemaAux.
 
     
   End TypePredicates.
+
+  (** ---- *)
+  (** *** Predicates about types *)
+  Section ValuePredicates.
+    
+    Variables (Scalar : eqType)
+              (s : graphQLSchema)
+              (is_valid_scalar_value : graphQLSchema -> Name -> Scalar -> bool).
+
+    (** ---- *)
+    (**
+       Checks whether the given value matches the expected type in the schema. 
+       To determine scalar values, the [is_valid_scalar_value] predicate must be 
+       provided.
+     *)
+    Equations is_valid_value (ty : type) (value : @Value Scalar) : bool :=
+      {
+        is_valid_value (NamedType n) (SValue value) := is_valid_scalar_value s n value;
+        is_valid_value (ListType wty) (LValue ls) := all (is_valid_value wty) ls;
+        is_valid_value _ _ := false
+      }.
+
+  End ValuePredicates.
+
+  Arguments is_valid_value [Scalar].
   
 
   (** ---- *)
